theories/Spilling/SpillMinKill.v
@@ -1,7 +1,7 @@
 Require Import List Map Env AllInRel Exp MoreList.
 Require Import IL Annotation.
 Require Import Liveness.Liveness.
-Require Import ExpVarsBounded SpillSound OneOrEmpty.
+Require Import ExpVarsBounded SpillSound OneOrEmpty RegLive.
 Require Import Take TakeSet.
 
 
@@ -17,6 +17,7 @@ Inductive spill_min_kill (k:nat) :
   -> (list (⦃var⦄ * ⦃var⦄))
   -> (⦃var⦄ * ⦃var⦄)
   -> stmt
+  -> ann ⦃var⦄
   -> spilling
   -> Prop
   :=
@@ -24,56 +25,61 @@ Inductive spill_min_kill (k:nat) :
   | SpillLet
       (ZL : list params)
       (Λ : list (⦃var⦄ * ⦃var⦄))
-      (R M Sp L K Kx : ⦃var⦄)
+      (R M Sp L Rlv : ⦃var⦄)
       (x : var)
       (e : exp)
       (s : stmt)
       (sl : spilling)
-    : Sp ⊆ R
+      (rlv : ann ⦃var⦄)
+    : let K := set_take_avoid (cardinal (R ∪ L) - k) (R \ Exp.freeVars e) (getAnn rlv) in
+      let Kx:= set_take_avoid (1 + cardinal (R \ K ∪ L) - k) (R \ K ∪ L) (getAnn rlv) in
+      Sp ⊆ R
       -> L ⊆ Sp ∪ M
-      -> spill_min_kill k ZL Λ ({x;(R\K ∪ L)\Kx }, Sp ∪ M) s sl
+      -> spill_min_kill k ZL Λ ({x;(R\K ∪ L)\Kx }, Sp ∪ M) s rlv sl
       -> Exp.freeVars e ⊆ R\K ∪ L
       -> k > 0
       -> cardinal (R\K ∪ L) <= k
       -> cardinal ({x;((R\K) ∪ L)\Kx }) <= k
-      -> spill_min_kill k ZL Λ (R,M) (stmtLet x e s) (ann1 (Sp,L,nil) sl)
-
+      -> spill_min_kill k ZL Λ (R,M) (stmtLet x e s) (ann1 Rlv rlv) (ann1 (Sp,L,nil) sl)
+                       
   | SpillReturn
       (ZL : list (params))
       (Λ : list (⦃var⦄ * ⦃var⦄))
-      (R M Sp L K : ⦃var⦄)
+      (R M Sp L Rlv: ⦃var⦄)
       (e : op)
-    : Sp ⊆ R
+    : let K := set_take (cardinal (R ∪ L) - k) (R \ Op.freeVars e) in 
+      Sp ⊆ R
       -> L ⊆ Sp ∪ M
       -> Op.freeVars e ⊆ R\K ∪ L
       -> cardinal ((R\K) ∪ L) <= k
-      -> spill_min_kill k ZL Λ (R,M) (stmtReturn e)
-                    (ann0 (Sp,L,nil))
+      -> spill_min_kill k ZL Λ (R,M) (stmtReturn e) (ann0 Rlv) (ann0 (Sp,L,nil))
 
   | SpillIf
       (ZL : list (params))
       (Λ : list (⦃var⦄ * ⦃var⦄))
-      (R M Sp L K : ⦃var⦄)
+      (R M Sp L Rlv: ⦃var⦄)
       (e : op)
       (s t : stmt)
       (sl_s sl_t : spilling)
-
-    : Sp ⊆ R
+      (rlv1 rlv2 : ann ⦃var⦄)
+    : let K := set_take_avoid (cardinal (R ∪ L) - k) (R \ Op.freeVars e ) (getAnn rlv1 ∪ getAnn rlv2) in
+      Sp ⊆ R
       -> L ⊆ Sp ∪ M
       -> Op.freeVars e ⊆ R\K ∪ L
       -> cardinal (R\K ∪ L) <= k
-      -> spill_min_kill k ZL Λ (R\K ∪ L, Sp ∪ M) s sl_s
-      -> spill_min_kill k ZL Λ (R\K ∪ L, Sp ∪ M) t sl_t
-      -> spill_min_kill k ZL Λ (R,M) (stmtIf e s t) (ann2 (Sp,L,nil) sl_s sl_t)
+      -> spill_min_kill k ZL Λ (R\K ∪ L, Sp ∪ M) s rlv1 sl_s
+      -> spill_min_kill k ZL Λ (R\K ∪ L, Sp ∪ M) t rlv2 sl_t
+      -> spill_min_kill k ZL Λ (R,M) (stmtIf e s t) (ann2 Rlv rlv1 rlv2) (ann2 (Sp,L,nil) sl_s sl_t)
 
   | SpillApp
       (ZL : list params)
       (Λ : list (⦃var⦄ * ⦃var⦄))
-      (R M Sp L K R_f M_f R' M' : ⦃var⦄)
+      (R M Sp L R_f M_f R' M' Rlv : ⦃var⦄)
       (f : lab)
       (Z : params)
       (Y : args)
-    : Sp ⊆ R
+    : let K := set_take (cardinal (R ∪ L) - k) (R \ R_f) in
+      Sp ⊆ R
       -> L ⊆ Sp ∪ M
       -> cardinal (R\K ∪ L) <= k
       -> get ZL (counted f) Z
@@ -82,31 +88,54 @@ Inductive spill_min_kill (k:nat) :
       -> M_f \ of_list Z ⊆ Sp ∪ M
       -> list_union (Op.freeVars ⊝ Y) ⊆ (R\K ∪ L) ∪ M'
       -> M' ⊆ Sp ∪ M
-      -> spill_min_kill k ZL Λ (R,M) (stmtApp f Y)
-                       (ann0 (Sp,L, (R', M')::nil))
+      -> spill_min_kill k ZL Λ (R,M) (stmtApp f Y) (ann0 Rlv) (ann0 (Sp,L, (R', M')::nil))
 
   | SpillFun
       (ZL : list params)
       (Λ rms : list (⦃var⦄ * ⦃var⦄))
-      (R M Sp L K : ⦃var⦄)
+      (R M Sp L Rlv : ⦃var⦄)
       (F : list (params * stmt))
       (t : stmt)
       (sl_F : list spilling)
       (sl_t : spilling)
-    : Sp ⊆ R
+      (rlv_t : ann ⦃var⦄)
+      (rlv_F : list (ann ⦃var⦄))
+    : let K := set_take_avoid (cardinal (R ∪ L) - k) R (getAnn rlv_t) in
+      Sp ⊆ R
       -> L ⊆ Sp ∪ M
       -> cardinal (R\K ∪ L) <= k
       -> length F = length sl_F
       -> length F = length rms
       -> (forall n rm, get rms n rm -> cardinal (fst rm) <= k)
-      -> (forall n Zs rm sl_s, get rms n rm
+      -> (forall n Zs rm rlv_s sl_s, get rms n rm
                          -> get F n Zs
+                         -> get rlv_F n rlv_s
                          -> get sl_F n sl_s
                          -> spill_min_kill k ((fst ⊝ F) ++ ZL)
-                                          (rms ++ Λ) rm (snd Zs) sl_s
+                                          (rms ++ Λ) rm (snd Zs) rlv_s sl_s
         )
-      -> spill_min_kill k ((fst ⊝ F) ++ ZL) (rms ++ Λ) (R\K ∪ L, Sp ∪ M) t sl_t
-      -> spill_min_kill k ZL Λ (R,M) (stmtFun F t)
-                       (annF (Sp,L,rms) sl_F sl_t)
+      -> spill_min_kill k ((fst ⊝ F) ++ ZL) (rms ++ Λ) (R\K ∪ L, Sp ∪ M) t rlv_t sl_t
+      -> spill_min_kill k ZL Λ (R,M) (stmtFun F t) (annF Rlv rlv_F rlv_t) (annF (Sp,L,rms) sl_F sl_t)
 .
+
+
+Lemma spill_sound_spill_min_kill k ZL Λ R R' M s sl rlv :
+  spill_sound k ZL Λ (R,M) s sl
+  -> rlive_sound ZL (fst ⊝ Λ) s sl rlv
+  -> getAnn rlv ⊆ R'
+  -> spill_min_kill k ZL Λ (R',M) s rlv sl
+.
+Proof.
+  intros spillSnd rlive rlv_sub. general induction spillSnd; invc rlive; cbn in rlv_sub.
+  - econstructor; eauto;
+      set (K' := set_take_avoid (cardinal (R' ∪ L) - k) (R' \ Exp.freeVars e) (getAnn al));
+      set (Kx':= set_take_avoid (1 + cardinal (R' \ K' ∪ L) - k) (R' \ K' ∪ L) (getAnn al)).
+    + admit. (* Sp ⊆ getAnn rlv Lemma *)
+    + eapply IHspillSnd; eauto. admit. (* disj (set_take_avoid s t) t Lemma *)
+    + rewrite <-rlv_sub. admit. (* solvable *)
+    + admit. (* Lemma *)
+    + admit. (* analogous *)
+  -           
+  
+      
 
