theories/Spilling/RepairSpillInv.v
@@ -10,13 +10,12 @@ Set Implicit Arguments.
 Lemma repair_spill_inv k ZL Λ s lv sl R M G
   : live_sound Imperative ZL (merge ⊝ Λ) s lv
     -> spill_sound k ZL Λ (R,M) s sl
-    -> sl === repair_spill k ZL Λ R M s lv (reg_live (fst ⊝ Λ) ZL G s sl) sl
+    -> sl === repair_spill k ZL Λ R M s lv (reg_live ZL (fst ⊝ Λ) G s sl) sl
 .
 Proof.
   intros liveSnd spillSnd.
   general induction sl; invc liveSnd; invc spillSnd; econstructor.
-  - econstructor; econstructor; symmetry;
-      apply inter_subset_equal in H9; apply inter_subset_equal in H10;
+  - assert (H10' := H10). assert (H9' := H9).
     assert (set_take_prefer k (L ∩ (Sp ∩ R ∪ M))
                               ((fst (nth (counted l) Λ ({},{}))
                                     \ of_list (nth (counted l) ZL nil)) \ R) [=] L) as Leq.
@@ -25,38 +24,46 @@ Proof.
       rewrite H9, H10. apply union_subset_equal;
             rewrite H16; clear; cset_tac).*)
     }
-    + rewrite H9 at 2. apply union_subset_equal. rewrite set_take_incl at 1. rewrite Leq.
+    econstructor; econstructor; symmetry;
+      apply inter_subset_equal in H9; apply inter_subset_equal in H10.
+    + rewrite Leq. rewrite H9. apply union_subset_equal.
       erewrite !get_nth; eauto. unfold fst,snd. rewrite H17.
       apply union_incl_split; [|clear;cset_tac].
-      apply meet_incl. 
-      rewrite H17. clear; cset_tac.
-    + erewrite !get_nth; eauto. unfold fst. apply Leq.
-    + erewrite !get_nth; eauto. unfold snd, fst. econstructor; eauto.
-      apply union_subset_equal. rewrite Leq.
-      rewrite meet_comm; apply meet_incl. rewrite H18.
-      enough (R \ K ∪ L [<=] R \ set_take (cardinal (R ∪ L) -k) (R \ R_f) ∪ L) as H'.
-      rewrite H'. clear. cset_tac. admit. (*
-      unfold set_take; rewrite take_set_incl. rewrite minus_minus.
-      rewrite meet_comm. apply meet_incl. rewrite Leq. rewrite H18, H9, H10. rewrite minus_minus.
-      assert (forall s t u : ⦃var⦄, s \ (s \ t)
-      apply incl_eq.
-      * admit.
-      * rewrite H17. apply union_incl_split.
-        -- clear; cset_tac.
-        -- rewrite H9 at 2. rewrite H10. unfold set_take. rewrite take_set_incl.
-           rewrite H18. rewrite H16.*)
-
-    + econstructor; eauto.      
-  - econstructor; econstructor; symmetry; apply inter_subset_equal in H6;
+      rewrite H18, H19. rewrite H10' at 1.
+      assert (K [=] set_take (cardinal (R ∪ L) - k) (R \ R_f)) as Keq by admit.
+      rewrite <-Keq.
+      clear; cset_tac.
+    + apply Leq. 
+    + rewrite Leq. erewrite !get_nth; eauto. unfold snd, fst. econstructor; eauto.
+      setoid_rewrite inter_subset_equal at 2; eauto. apply union_subset_equal.
+      assert (K [=] set_take (cardinal (R ∪ L) - k) (R \ R_f)) as Keq by admit.
+      rewrite <-Keq.
+      rewrite H18. clear; cset_tac.
+    + econstructor; eauto.
+  - assert (H6' := H6).
+    econstructor; econstructor; apply inter_subset_equal in H6;
       eauto.
-    assert (Op.freeVars e \ R ∪ (L ∩ (Sp ∩ R ∪ M)) [=] L) as Hypo.
+    assert ((L ∩ (Sp ∩ R ∪ M)) [=] L) as Leq.
     {
-      apply inter_subset_equal in H7. rewrite H6, H7. apply union_subset_equal.
-      clear - H8. cset_tac.
+      apply inter_subset_equal in H7. rewrite H6, H7. eauto.
     }
     rewrite set_take_prefer_eq; eauto.
-    rewrite Hypo. rewrite subset_cardinal with (s':=R \ K ∪ L); eauto; clear; cset_tac.
-  - econstructor; econstructor; symmetry;
+    + rewrite Leq. rewrite subset_cardinal; eauto.
+    + rewrite H8, Leq. clear; cset_tac.
+  - assert (H12' := H12); assert (H13' := H13).
+    assert (Sp ∩ R [=] Sp) as Speq'
+        by (apply inter_subset_equal; eauto).
+    assert (L ∩ (Sp ∩ R ∪ M) [=] L) as Leq'
+        by (rewrite Speq'; apply inter_subset_equal; rewrite  H13; eauto).
+    assert (set_take_prefer k (L ∩ (Sp ∩ R ∪ M)) (Exp.freeVars e \ R) [=] L) as Leq.
+    {
       apply inter_subset_equal in H12; apply inter_subset_equal in H13.
-    + rewrite H12 at 6. apply union_subset_equal. admit. 
-    + rewrite H12, H13. apply union_subset_equal. clear - H15; cset_tac.
+      rewrite set_take_prefer_eq; eauto; rewrite Leq'.
+      - rewrite subset_cardinal; [apply H17|]; eauto.
+      - rewrite H15; clear; cset_tac.
+    }
+    econstructor; econstructor; symmetry;
+      apply inter_subset_equal in H12; apply inter_subset_equal in H13.
+    + admit.
+    + apply Leq.
+      
